ulib/experimental/Steel.FractionalPermission.fst
@@ -1,14 +1,9 @@
 module Steel.FractionalPermission
 open FStar.Real
-open Steel.PCM
 
-#set-options "--fuel 0 --ifuel 1"
-
-[@erasable]
-noeq type perm : Type u#0 =
-  | MkPerm: v:real{v >. 0.0R} -> perm
-
-let full_perm : perm = MkPerm 1.0R
+[@@erasable]
+noeq type perm : Type0 =
+  | MkPerm: v:real{ v >. 0.0R } -> perm
 
 let writeable (p: perm) : GTot bool =
   MkPerm?.v p = 1.0R
@@ -22,36 +17,4 @@ let sum_perm (p1 p2: perm) : Tot perm =
 let lesser_equal_perm (p1 p2:perm) : GTot bool =
   MkPerm?.v p1 <=.  MkPerm?.v p2
 
-noeq type with_perm (a: Type u#a) = {
-  value: a;
-  perm: perm
-}
-
-let composable_with_perm' (#a: Type) (x y: with_perm a) : prop =
-  x.value == y.value /\
-  lesser_equal_perm (sum_perm x.perm y.perm) full_perm
-
-let composable_with_perm (#a: Type) : symrel (with_perm a) =
-  fun (x y: with_perm a) -> composable_with_perm' x y
-
-
-let compose_with_perm
-  (#a: Type u#a)
-  (x: with_perm a)
-  (y: with_perm a{x `composable_with_perm ` y}) =
-  {
-   value = x.value;
-   perm = sum_perm x.perm y.perm
-  }
-
-let frac_perm_pcm' (#a: Type u#a) : unitless_pcm' (with_perm a) = {
-  unitless_composable = composable_with_perm;
-  unitless_op = compose_with_perm;
-}
-
-let frac_perm_pcm (#a: Type u#a) : unitless_pcm (with_perm a) = {
-  unitless_p = frac_perm_pcm';
-  unitless_comm = (fun _ _ -> ());
-  unitless_assoc = (fun _ _ _ -> ());
-  unitless_assoc_r = (fun _ _ _ -> ());
-}
+let full_perm : perm = MkPerm 1.0R
